SciLean/Core/Monads/ForIn.lean
@@ -1,5 +1,6 @@
 import SciLean.Core.Monads.FwdDerivMonad
 import SciLean.Core.Monads.Id
+import SciLean.Data.DataArray
 
 set_option linter.unusedVariables false
 
@@ -8,17 +9,15 @@ namespace SciLean
 variable 
   {K : Type _} [IsROrC K]
   
--- This is not true but lets assume it for now until I have 
+-- This is not true but lets assume it for now
 instance [Vec K X] : Vec K (ForInStep X) := sorry
 
--- This is not true but lets assume it for now until I have 
+-- This is not true but lets assume it for now
 instance [SemiInnerProductSpace K X] : SemiInnerProductSpace K (ForInStep X) := sorry
 
 
 end SciLean
 open SciLean
-
--- set_option linter.unusedVariables false
 
 def ForInStep.val : ForInStep α → α
 | .yield a => a
@@ -60,6 +59,9 @@ variable
   {Y : Type _} [Vec K Y]
   {Z : Type _} [Vec K Z]
 
+--------------------------------------------------------------------------------
+-- ForIn.forIn -----------------------------------------------------------------
+--------------------------------------------------------------------------------
 
 -- we need some kind of lawful version of `ForIn` to be able to prove this
 @[fprop]
@@ -101,6 +103,9 @@ by
   simp [forIn,Std.Range.forIn,Std.Range.forIn.loop,Std.Range.forIn.loop.match_1]
   ftrans
 
+--------------------------------------------------------------------------------
+-- ForInStep.yield -------------------------------------------------------------
+--------------------------------------------------------------------------------
 
 @[fprop]
 theorem ForInStep.yield.arg_a0.IsDifferentiable_rule
@@ -133,6 +138,11 @@ theorem ForInStep.done.arg_a0.IsDifferentiable_rule
   (a0 : X → Y) (ha0 : IsDifferentiable K a0)
   : IsDifferentiable K fun x => ForInStep.done (a0 x) := by sorry_proof
 
+
+--------------------------------------------------------------------------------
+-- ForInStep.done -------------------------------------------------------------
+--------------------------------------------------------------------------------
+
 -- this is a hack as with Id monad sometimes you do not need `pure` which trips `fprop` up
 @[fprop]
 theorem ForInStep.done.arg_a0.IsDifferentiableM_rule
@@ -157,6 +167,8 @@ theorem ForInStep.done.arg_a0.fwdCDeriv_rule
 end OnVec
 
 
+--------------------------------------------------------------------------------
+
 
 section OnSemiInnerProductSpace
 
@@ -168,7 +180,12 @@ variable
   {X : Type _} [SemiInnerProductSpace K X]
   {Y : Type _} [SemiInnerProductSpace K Y]
   {Z : Type _} [SemiInnerProductSpace K Z]
+  {W : Type _} [SemiInnerProductSpace K W]
 
+
+--------------------------------------------------------------------------------
+-- ForIn.forIn -----------------------------------------------------------------
+--------------------------------------------------------------------------------
 
 -- we need some kind of lawful version of `ForIn` to be able to prove this
 @[fprop]
@@ -177,10 +194,18 @@ theorem ForIn.forIn.arg_bf.HasAdjDiffM_rule
   (hinit : HasAdjDiff K init) (hf : ∀ a, HasAdjDiffM K (fun (xy : X×Y) => f xy.1 a xy.2))
   : HasAdjDiffM K (fun x => forIn range (init x) (f x)) := sorry_proof
 
+@[fprop]
+theorem ForIn.forIn.arg_bf.HasAdjDiff_rule [ForIn Id ρ α]
+  (range : ρ) (init : X → Y) (f : X → α → Y → (ForInStep Y))
+  (hinit : HasAdjDiff K init) (hf : ∀ a, HasAdjDiff K (fun (xy : X×Y) => f xy.1 a xy.2))
+  : HasAdjDiff K (fun x => forIn (m:=Id) range (init x) (f x)) := sorry_proof
 
--- we need some kind of lawful version of `ForIn` to be able to prove this
-@[ftrans]
-theorem ForIn.forIn.arg_bf.revDerivM_rule
+
+/-- This version of reverse derivative of a for loop builds a big lambda function
+  for the reverse pass during the forward pass. This is probably ok in for loops
+  where each iteration is very costly and there are not many iterations.
+-/
+theorem ForIn.forIn.arg_bf.revDerivM_rule_lazy
   (range : ρ) (init : X → Y) (f : X → α → Y → m (ForInStep Y))
   (hinit : HasAdjDiff K init) (hf : ∀ a, HasAdjDiffM K (fun (xy : X×Y) => f xy.1 a xy.2))
   : revDerivM K (fun x => forIn range (init x) (f x)) 
@@ -205,55 +230,117 @@ theorem ForIn.forIn.arg_bf.revDerivM_rule
 by
   sorry_proof
 
-theorem ForIn.forIn.arg_bf.revDerivM_rule_alternative [ForIn Id ρ α]
-  (init : X → Y) (f : X → Nat → Y → Y)
-  (hinit : HasAdjDiff K init) (hf : ∀ a, HasAdjDiff K (fun (xy : X×Y) => f xy.1 a xy.2))
-  : revDerivM K (fun x => forIn (m:=Id) (Std.Range.mk start stop step) (init x) (fun i y => .yield (f x i y))) 
+
+/-- Reverse pass of a for loop implemented using `DataArray`
+
+  See `Forin.arg_bf.revCDeriv_rule_dataArrayImpl` how it relates to reverse derivative of for loop.
+
+  TODO: Index shoud support iterating in reverse order
+
+  WARNING: `dx'` and `dw` behave differently
+     - `df'` computes gradient in `dx'` 
+     - `df'` computes update to gradient in `dw` 
+  
+  The value of `df'` should be:
+    df' = fun w i x dx' dw => 
+      ((∇ (x':=x;dx'), f w i x'), (dw + ∇ (w':=w;dx'), f w' i x))
+  -/
+def ForIn.arg_bf.revPass_dataArrayImpl [Index ι] [PlainDataType X] [PlainDataType W] [Zero X] [Zero W]
+  (df' : W → ι → X → X → W → X×W) (w : W) (xs : DataArrayN X ι) (dx' : X) : X×W := Id.run do
+  let n := Index.size ι
+  let mut dx' := dx'
+  let mut dw : W := 0
+  for i in [0:n.toNat] do
+    let j : ι := fromIdx ⟨n-i.toUSize-1,sorry_proof⟩
+    let xj := xs[j]
+    let dxw' := df' w j xj dx' dw
+    dx' := dxw'.1
+    dw := dxw'.2
+  (dx',dw)
+
+
+/-- Reverse derivative of a for loop
+
+  WARNING: `dx'` and `dw` behave differently
+     - `df'` computes gradient in `dx'` 
+     - `df'` computes update to gradient in `dw` 
+  
+  The value of `df'` should be:
+    df' = fun w i x dx' dw => 
+      ((∇ (x':=x;dx'), f w i x'), (dw + ∇ (w':=w;dx'), f w' i x))
+-/
+def ForIn.arg_bf.revDeriv_dataArrayImpl [Index ι] [PlainDataType X] [PlainDataType W] [Zero X] [Zero W]
+  (init : X) (f : W → ι → X → X) (df' : W → ι → X → X → W → X×W) (w : W)
+  : X×(X→X×W) :=
+  Id.run do
+    let n := Index.size ι
+    -- forward pass
+    let mut xs : DataArray X := .mkEmpty n
+    let mut x := init
+    for i in fullRange ι do
+      xs := xs.push x
+      x := f w i x
+    let xs' : DataArrayN X ι := ⟨xs, sorry_proof⟩
+    (x, fun dx' => ForIn.arg_bf.revPass_dataArrayImpl df' w xs' dx')
+
+
+/-- The do notation leaves the for loop body in a strange form `do pure PUnit.unit; pure <| ForInStep.yield (f w i y))`
+  Marking this theorem with `ftrans` is a bit of a hack. It normalizes the body to `ForInStep.yield (f w i y)`.
+  -/
+@[ftrans]
+theorem ForIn.forIn.arg_bf.revDerivM_rule_normalization [Index ι]
+  (init : W → X) (f : W → ι → X → X)
+  : revDerivM K (fun w => forIn (m:=Id) (fullRange ι) (init w) (fun i y => do pure PUnit.unit; pure <| ForInStep.yield (f w i y)))
     =
-    (fun x => Id.run do
-      let (y₀,dinit') := revCDeriv K init x
-      let (y,ys) ← forIn (Std.Range.mk start stop step) (y₀,#[]) (fun i (y,ys) => 
-        let y' := f x i y
-        .yield (y', ys.push y'))
-      pure (y, 
-            fun dy => do
-              let (dx,dy) ← forIn (Std.Range.mk start stop step) ((0:X),dy) (fun i (dx,dy) => do 
-                let j := stop - ((i-start) + 1)
-                let yᵢ : Y := ys[j]!
-                let (dx',dy) := (revCDeriv K (fun (xy : X×Y) => f xy.1 i xy.2) (x,yᵢ)).2 dy
-                .yield (dx + dx', dy))
-              pure (dx + dinit' dy))) :=
+    revCDeriv K (fun w => forIn (m:=Id) (fullRange ι) (init w) (fun i y => ForInStep.yield (f w i y))) := by rfl
+
+
+
+/-- The do notation leaves the for loop body in a strange form `do pure PUnit.unit; pure <| ForInStep.yield (f w i y))`
+  Marking this theorem with `ftrans` is a bit of a hack. It normalizes the body to `ForInStep.yield (f w i y)`.
+  -/
+@[ftrans]
+theorem ForIn.forIn.arg_bf.revCDeriv_rule_normalization [Index ι]
+  (init : W → X) (f : W → ι → X → X)
+  : revCDeriv K (fun w => forIn (m:=Id) (fullRange ι) (init w) (fun i y => do pure PUnit.unit; pure <| ForInStep.yield (f w i y)))
+    =
+    revCDeriv K (fun w => forIn (m:=Id) (fullRange ι) (init w) (fun i y => ForInStep.yield (f w i y))) := by rfl
+
+
+@[ftrans]
+theorem ForIn.forIn.arg_bf.revCDeriv_rule_def [Index ι] [PlainDataType X] [PlainDataType W]
+  (init : W → X) (f : W → ι → X → X)
+  (hinit : HasAdjDiff K init) (hf : ∀ i, HasAdjDiff K (fun (w,x) => f w i x))
+  : revCDeriv K (fun w => forIn (m:=Id) (fullRange ι) (init w) (fun i y => ForInStep.yield (f w i y)))
+    =
+    fun w => (Id.run do
+      let n := Index.size ι
+      let initdinit := revCDeriv K init w
+
+      -- forward pass
+      let mut xs : DataArray X := .mkEmpty n
+      let mut x := initdinit.1
+      for i in fullRange ι do
+        xs := xs.push x
+        x := f w i x
+      let xs' : DataArrayN X ι := ⟨xs, sorry_proof⟩
+
+      let revPassBody := hold fun w i x dx' dw =>
+        let dwx' := gradient K (fun (w',x') => f w' i x') (w,x) dx'
+        (dwx'.2, dw + dwx'.1)
+
+      (x, 
+       fun dx' =>
+         -- reverse pass
+         let dxw' := ForIn.arg_bf.revPass_dataArrayImpl revPassBody w xs' dx'
+         initdinit.2 dxw'.1 + dxw'.2)) :=
 by
   sorry_proof
 
   
-
--- Proof that the above theorem is true for the range [0:3] and function that does not break the for loop
-example
-  (init : X → Y) (f : X → Nat → Y → m Y)
-  (hinit : HasAdjDiff K init) (hf : ∀ a, HasAdjDiffM K (fun (xy : X×Y) => f xy.1 a xy.2))
-  : revDerivM K (fun x => forIn [0:3] (init x) (fun i y => do pure (ForInStep.yield (← f x i y)))) 
-    = 
-    (fun x => do
-      let ydinit := revCDeriv K init x
-      let ydf ← forIn [0:3] (ydinit.1, fun (dy:Y) => pure (f:=m') ((0:X),dy))
-        (fun a ydf => do
-          let ydf' ← revDerivM K (fun (xy : X×Y) => f xy.1 a xy.2) (x,ydf.1)
-          let df : Y → m' (X×Y) := 
-            fun dy : Y => do
-              let dxy  ← ydf'.2 dy
-              let dxy' ← ydf.2 dxy.2
-              pure (dxy.1 + dxy'.1, dxy'.2)
-          pure (ForInStep.yield (ydf'.1, df)))
-      pure (ydf.1, 
-            fun dy => do
-              let dxy ← ydf.2 dy
-              pure (dxy.1 + ydinit.2 dxy.2))) :=
-by
-  simp [revCDeriv,forIn,Std.Range.forIn,Std.Range.forIn.loop,Std.Range.forIn.loop.match_1, revCDeriv]
-  ftrans
-  simp[add_assoc, revCDeriv]
-
+--------------------------------------------------------------------------------
+-- ForInStep.yield -------------------------------------------------------------
+--------------------------------------------------------------------------------
 
 @[fprop]
 theorem ForInStep.yield.arg_a0.HasAdjDiff_rule
@@ -315,4 +402,9 @@ theorem ForInStep.done.arg_a0.revDerivM_rule
       (.done ydf.1, fun y => ydf.2 y.val)
   := by sorry_proof
 
+
 end OnSemiInnerProductSpace
+
+
+
+
