SciLean/Core/Monads/ForInTests.lean
@@ -1,5 +1,7 @@
 import SciLean.Core.Monads.ForIn
 import SciLean.Tactic.LetNormalize
+import SciLean.Core.FloatAsReal
+import SciLean.Core.Notation
 
 open SciLean
 
@@ -12,6 +14,7 @@ variable
   {X : Type _} [Vec K X]
   {Y : Type _} [Vec K Y]
   {Z : Type _} [Vec K Z]
+
 
 -- 
 set_option pp.notation false in
@@ -70,12 +73,55 @@ example : fwdDerivM K (fun x : K => show m K from do
     pure ydy)
   := 
 by
-  (conv => lhs; ftrans only; let_normalize; ftrans only; simp (config := {zeta := false}))
+  (conv => lhs; ftrans; ftrans; simp (config := {zeta := false}))
   simp
-  funext x dx
-  congr
-  funext a (y,dy)
-  simp
+
+-- @[ftrans_simp]
+-- theorem revDerivM_eq_revCDeriv_on_Id' 
+--   [SemiInnerProductSpace K X] [SemiInnerProductSpace K Y] (x : X) (f : X → Y)
+--   : revDerivM K fun f = revCDeriv K f := by set_option pp.all true in rfl
+
+
+#eval
+  ((gradient Float (fun x : Float ^ Idx 3 => Id.run do
+    let mut y := 1.0
+    for i in fullRange (Idx 3) do
+      y := y * x[i]
+    y))
+    rewrite_by
+      unfold gradient
+      ftrans
+      ftrans
+      ftrans
+      unfold gradient
+      ftrans)
+  ⊞[5.0,6,7] 1
+
+variable (y y' : Id Float × (Id Float → Float)) (b' : Id Float × (Id Float → Float) → Float) (b : Float × (Float → Float) → Float) (q : y' = y)  (h : ∀ (x : Id Float × (Id Float → Float)), x = y → let z : Float × (Float → Float) := x; (b z = b' z))
+
+#check Tactic.LSimp.let_congr_eq (α := Float × (Float → Float)) q h
+
+set_option trace.Meta.Tactic.simp.discharge true in
+set_option trace.Meta.Tactic.fprop.discharge true in
+-- set_option trace.Meta.Tactic.fprop.step true in
+set_option trace.Meta.Tactic.ftrans.step true in
+set_option pp.notation false in
+#eval
+  ((gradient Float (fun x : Float ^ Idx 10 => Id.run do
+    let mut s := x[(⟨0,sorry⟩ : Idx 10)]
+    for i in [0:9] do
+      let i : Idx 10 := ⟨i.toUSize+1,sorry⟩
+      s := s + x[i]
+    s))
+    rewrite_by
+      unfold gradient
+      ftrans
+      ftrans
+      ftrans
+      unfold gradient
+      ftrans)
+  ⊞[5.0,6,7,8,9,10,11,12,13,14] 1
+
 
 -- example : fwdDerivM K (fun x : K => show m K from do
 --   let mut y := x
